Move seq helper functions

fstar/Syntax.fst
@@ -18,3 +18,10 @@ type com =
  | Sequence : s1:com -> s2:com -> com
  | If : cond:exp -> thn:com -> els:com -> com
  | While : cond:exp -> body:com -> com
+
+
+// Easier way to write sequences of commands
+val seq : list com -> com
+let rec seq ss = match ss with
+ | [] -> Skip
+ | hd :: tl -> Sequence hd (seq tl)
